ott_coq/destination_calculus_proofs.v
@@ -4,93 +4,104 @@ Require Import Ott.destination_calculus_ott.
 Require Import Ott.destination_calculus_notations.
 Require Import Ott.ext_nat.
 Require Import Coq.Program.Equality.
+Require Import Ott.Finitely.
+From Hammer Require Import Hammer.
 From Hammer Require Import Tactics.
 
-(* Todo : add equivalences *)
-
-(* Define Ltac macro to prove ctx lemma easily *)
-
-Lemma ValidUnionBackward : forall (G1 G2 : ctx), ctx_IsValid (G1 ⨄ G2) -> ctx_IsValid G1 /\ ctx_IsValid G2. Proof. Admitted.
-Lemma ValidUnionForward : forall (G1 G2 : ctx), ctx_IsValid G1 -> ctx_IsValid G2 -> ctx_Disjoint G1 G2 -> ctx_IsValid (G1 ⨄ G2). Proof. Admitted.
-Lemma ValidStimesBackward : forall (m : mode) (G : ctx), ctx_IsValid (m ᴳ· G) -> ctx_IsValid G /\ mode_IsValid m. Proof. Admitted.
-Lemma ValidStimesForward : forall (m : mode) (G : ctx), mode_IsValid m -> ctx_IsValid G -> ctx_IsValid (m ᴳ· G). Proof. Admitted.
-Lemma ValidMinusBackward : forall (G : ctx), ctx_IsValid (ᴳ-G) -> ctx_IsValid G. Proof. Admitted.
-Lemma ValidMinusForward : forall (G : ctx), ctx_IsValid G -> ctx_IsValid (ᴳ-G). Proof. Admitted.
-Lemma DestOnlyUnionBackward : forall (G1 G2 : ctx), ctx_DestOnly (G1 ⨄ G2) -> ctx_DestOnly G1 /\ ctx_DestOnly G2.
+Lemma ValidOnlyUnionBackward : forall (G1 G2 : ctx), ctx_ValidOnly (G1 ⨄ G2) -> ctx_ValidOnly G1 /\ ctx_ValidOnly G2.
 Proof. Admitted.
-Lemma DestOnlyUnionForward : forall (G1 G2 : ctx), ctx_DestOnly G1 -> ctx_DestOnly G2 -> ctx_DestOnly (G1 ⨄ G2).
+Lemma ValidOnlyUnionForward : forall (G1 G2 : ctx), ctx_ValidOnly G1 -> ctx_ValidOnly G2 -> ctx_Disjoint G1 G2 -> ctx_ValidOnly (G1 ⨄ G2).
 Proof. Admitted.
-Lemma DestOnlyStimesForward : forall (m : mode) (G : ctx), ctx_DestOnly G -> ctx_DestOnly (m ᴳ· G).
+Lemma ValidOnlyStimesEquiv : forall (m : mode) (G : ctx), ctx_ValidOnly (m ᴳ· G) <-> ctx_ValidOnly G /\ mode_IsValid m.
 Proof. Admitted.
-Lemma DestOnlyStimesBackward : forall (m : mode) (G : ctx), ctx_DestOnly (m ᴳ· G) -> ctx_DestOnly G.
+Lemma ValidOnlyMinusEquiv : forall (G : ctx), ctx_ValidOnly (ᴳ-G) <-> ctx_LinNuOnly G /\ ctx_DestOnly G.
 Proof. Admitted.
-Lemma DestOnlyMinusForward : forall (G : ctx), ctx_DestOnly G -> ctx_DestOnly (ᴳ-G).
+Lemma DestOnlyUnionEquiv : forall (G1 G2 : ctx), ctx_DestOnly (G1 ⨄ G2) <-> ctx_DestOnly G1 /\ ctx_DestOnly G2.
 Proof. Admitted.
-Lemma DestOnlyMinusBackward : forall (G : ctx), ctx_DestOnly (ᴳ-G) -> ctx_DestOnly G.
-Proof. Admitted.
-Lemma LinOnlyUnionBackward : forall (G1 G2 : ctx), ctx_LinOnly (G1 ⨄ G2) -> ctx_LinOnly G1 /\ ctx_LinOnly G2 /\ ctx_Disjoint G1 G2.
-Proof. Admitted.
-Lemma LinOnlyUnionForward : forall (G1 G2 : ctx), ctx_LinOnly G1 -> ctx_LinOnly G2 -> ctx_Disjoint G1 G2 -> ctx_LinOnly (G1 ⨄ G2).
-Proof. Admitted.
-Lemma LinOnlyStimesBackward : forall (m : mode) (G : ctx), ctx_LinOnly (m ᴳ· G) -> ctx_LinOnly G /\ mode_IsLin m.
-Proof. Admitted.
-Lemma LinOnlyStimesForward : forall (m : mode) (G : ctx), ctx_LinOnly G -> mode_IsLin m -> ctx_LinOnly (m ᴳ· G).
-Proof. Admitted.
-Lemma LinOnlyMinusBackward : forall (G : ctx), ctx_LinOnly (ᴳ-G) -> ctx_LinOnly G.
-Proof. Admitted.
-Lemma LinOnlyMinusForward : forall (G : ctx), ctx_LinOnly G -> ctx_LinOnly (ᴳ-G).
+Lemma DestOnlyStimesEquiv : forall (m : mode) (G : ctx), ctx_DestOnly G <-> ctx_DestOnly (m ᴳ· G).
 Proof. Admitted.
 
-Lemma LinOnlyIsValid : forall (G : ctx), ctx_LinOnly G -> ctx_IsValid G.
+Lemma LinNuOnlyUnionEquiv : forall (G1 G2 : ctx), ctx_LinNuOnly (G1 ⨄ G2) <-> ctx_LinNuOnly G1 /\ ctx_LinNuOnly G2 /\ ctx_Disjoint G1 G2.
 Proof. Admitted.
-Lemma LinOnlyEmpty : ctx_LinOnly ᴳ{}.
+Lemma LinNuOnlyStimesEquiv : forall (m : mode) (G : ctx), ctx_LinNuOnly (m ᴳ· G) <-> ctx_LinNuOnly G /\ mode_IsLinNu m.
 Proof. Admitted.
-Lemma IsLinIsValid : forall (m : mode), mode_IsLin m -> mode_IsValid m. Proof.
+
+Lemma LinOnlyUnionEquiv : forall (G1 G2 : ctx), ctx_LinOnly (G1 ⨄ G2) <-> ctx_LinOnly G1 /\ ctx_LinOnly G2 /\ ctx_Disjoint G1 G2.
+Proof. Admitted.
+Lemma LinOnlyStimesEquiv : forall (m : mode) (G : ctx), ctx_LinOnly (m ᴳ· G) <-> ctx_LinOnly G /\ mode_IsLin m.
+Proof. Admitted.
+
+Lemma LinNuOnlyWkLinOnly : forall (G : ctx), ctx_LinNuOnly G -> ctx_LinOnly G.
+Proof. Admitted.
+Lemma LinOnlyWkValidOnly : forall (G : ctx), ctx_LinOnly G -> ctx_ValidOnly G.
+Proof. Admitted.
+
+Lemma IsLinNuWkIsLin : forall (m : mode), mode_IsLinNu m -> mode_IsLin m.
+Proof. Admitted.
+Lemma IsLinWkIsValid : forall (m : mode), mode_IsLin m -> mode_IsValid m. Proof.
   intros m H. destruct H. apply (mode_IsValidProof (Lin, a)).
 Qed.
-Lemma hdns_Disjoint_implies_Disjoint : forall (D D' : ctx) (C : ectxs) (T U0: type), D ⊣ C : T ↣ U0 -> hdns_Disjoint hnamesꟲ( C) hnamesᴳ(D') -> ctx_Disjoint D D'. Proof. Admitted.
-Lemma DisjointStimesLeftBackward : forall (m : mode) (D D' : ctx), ctx_Disjoint (m ᴳ· D) D' -> ctx_Disjoint D D'. Proof. Admitted.
-Lemma DisjointStimesRightBackward : forall (m : mode) (D D' : ctx), ctx_Disjoint D (m ᴳ· D') -> ctx_Disjoint D D'. Proof. Admitted.
-Lemma DisjointStimesLeftForward : forall (m : mode) (D D' : ctx), ctx_Disjoint D D' -> ctx_Disjoint (m ᴳ· D) D'. Proof. Admitted.
-Lemma DisjointStimesRightForward : forall (m : mode) (D D' : ctx), ctx_Disjoint D D' -> ctx_Disjoint D (m ᴳ· D'). Proof. Admitted.
-Lemma DisjointMinusLeftForward : forall (D D' : ctx), ctx_Disjoint D D' -> ctx_Disjoint (ᴳ-D) D'. Proof. Admitted.
-Lemma DisjointMinusRightForward : forall (D D' : ctx), ctx_Disjoint D D' -> ctx_Disjoint D (ᴳ-D'). Proof. Admitted.
-Lemma DisjointMinusLeftBackward : forall (D D' : ctx), ctx_Disjoint (ᴳ-D) D' -> ctx_Disjoint D D'. Proof. Admitted.
-Lemma DisjointMinusRightBackward : forall (D D' : ctx), ctx_Disjoint D (ᴳ-D') -> ctx_Disjoint D D'. Proof. Admitted.
-Lemma DisjointNestedLeft : forall (D D' D'' : ctx), ctx_Disjoint (D ⨄ D') D'' -> ctx_Disjoint D D'' /\ ctx_Disjoint D' D''. Proof. Admitted.
-Lemma DisjointNestedRight : forall (D D' D'' : ctx), ctx_Disjoint D  (D' ⨄ D'') -> ctx_Disjoint D D' /\ ctx_Disjoint D D''. Proof. Admitted.
 
-Lemma Ty_ectxs_DLin : forall (D : ctx) (C : ectxs) (T U0 : type), (D ⊣ C : T ↣ U0) -> ctx_LinOnly D.
+Lemma DisjointStimesLeftEquiv : forall (m : mode) (D D' : ctx), ctx_Disjoint (m ᴳ· D) D' <-> ctx_Disjoint D D'.
+Proof. Admitted.
+Lemma DisjointStimesRightEquiv : forall (m : mode) (D D' : ctx), ctx_Disjoint D (m ᴳ· D') <-> ctx_Disjoint D D'.
+Proof. Admitted.
+Lemma DisjointMinusLeftEquiv : forall (D D' : ctx), ctx_Disjoint D D' <-> ctx_Disjoint (ᴳ-D) D'.
+Proof. Admitted.
+Lemma DisjointMinusRightEquiv : forall (D D' : ctx), ctx_Disjoint D D' <-> ctx_Disjoint D (ᴳ-D').
+Proof. Admitted.
+Lemma DisjointNestedLeftEquiv : forall (D D' D'' : ctx), ctx_Disjoint (D ⨄ D') D'' <-> ctx_Disjoint D D'' /\ ctx_Disjoint D' D''.
+Proof. Admitted.
+Lemma DisjointNestedRightEquiv : forall (D D' D'' : ctx), ctx_Disjoint D  (D' ⨄ D'') <-> ctx_Disjoint D D' /\ ctx_Disjoint D D''.
+Proof. Admitted.
+
+Lemma hdns_DisjointImpliesDisjoint : forall (D D' : ctx) (C : ectxs) (T U0: type) (TyC: D ⊣ C : T ↣ U0) (DisjointCD': hdns_Disjoint hnamesꟲ( C) hnamesᴳ(D')), ctx_Disjoint D D'.
+Proof. Admitted.
+
+Lemma EmptyIsLinOnly : ctx_LinOnly ᴳ{}. (* TODO remove when we have actual definition of ctx_ValidOnly *)
+Proof. Admitted.
+
+Lemma EmptyUnionLeft : forall (G : ctx), G = G ⨄ ᴳ{}.
+Proof. Admitted.
+Lemma EmptyUnionRight : forall (G : ctx), G = ᴳ{} ⨄ G.
+Proof. Admitted.
+
+Lemma DisjointDestOnlyVar : forall (G : ctx) (x : var) (m : mode) (T : type), ctx_DestOnly G -> ctx_Disjoint G (ᴳ{ x : m ‗ T}).
+Proof. Admitted.
+
+Ltac hauto_ctx :=
+  hauto
+    depth: 3
+    use: ValidOnlyUnionBackward, ValidOnlyUnionForward, ValidOnlyStimesEquiv, ValidOnlyMinusEquiv, DestOnlyUnionEquiv, DestOnlyStimesEquiv, LinNuOnlyUnionEquiv, LinNuOnlyStimesEquiv, LinOnlyUnionEquiv, LinOnlyStimesEquiv, LinNuOnlyWkLinOnly, LinOnlyWkValidOnly, IsLinNuWkIsLin, IsLinWkIsValid, DisjointStimesLeftEquiv, DisjointStimesRightEquiv, DisjointMinusLeftEquiv, DisjointMinusRightEquiv, DisjointNestedLeftEquiv, DisjointNestedRightEquiv, hdns_DisjointImpliesDisjoint, EmptyIsLinOnly, EmptyUnionLeft, EmptyUnionRight, DisjointDestOnlyVar.
+
+Lemma Ty_ectxs_LinOnlyD : forall (D : ctx) (C : ectxs) (T U0 : type) (TyC: D ⊣ C : T ↣ U0), ctx_LinOnly D.
 Proof.
   intros D C T U0 H. induction H.
-  - apply LinOnlyEmpty.
-  - best use: LinOnlyUnionBackward use: LinOnlyStimesBackward.
-  - best use: LinOnlyUnionBackward use: LinOnlyStimesBackward.
-  - best use: LinOnlyUnionBackward use: LinOnlyStimesBackward.
-  - best use: LinOnlyUnionBackward use: LinOnlyStimesBackward.
-  - best use: LinOnlyUnionBackward use: LinOnlyStimesBackward.
-  - best use: LinOnlyUnionBackward use: LinOnlyStimesBackward.
-  - best use: LinOnlyUnionBackward use: LinOnlyStimesBackward.
-  - best use: LinOnlyUnionBackward use: LinOnlyStimesBackward.
-  - best use: LinOnlyUnionBackward use: LinOnlyStimesBackward.
-  - best use: LinOnlyUnionBackward use: LinOnlyStimesBackward.
-  - best use: LinOnlyUnionBackward use: LinOnlyStimesBackward.
-  - best use: LinOnlyUnionBackward use: LinOnlyStimesBackward.
-  - best use: LinOnlyUnionBackward use: LinOnlyStimesBackward.
-  - best use: LinOnlyUnionBackward use: LinOnlyStimesBackward.
-  - best use: LinOnlyUnionBackward use: LinOnlyStimesBackward.
-  - best use: LinOnlyUnionBackward use: LinOnlyStimesBackward.
-  - best use: LinOnlyUnionBackward use: LinOnlyStimesBackward.
-  - assert (ctx_LinOnly D2) as LinOnlyD2 by apply (LinOnlyUnionBackward D1 D2 IHTy_ectxs).
-    assert (ctx_LinOnly (¹↑ ᴳ· D2)) as LinOnlysD2 by apply (LinOnlyStimesForward ¹↑ D2 LinOnlyD2 (mode_IsLinProof (Fin 1))).
-    assert (ctx_Disjoint (D1 ⨄ D2) (ᴳ-D3)) by apply (hdns_Disjoint_implies_Disjoint (D1 ⨄ D2) (ᴳ-D3) C (T1 ⧔ U) U0 H H0).
-    assert (ctx_Disjoint D1 (ᴳ- D3) /\ ctx_Disjoint D2 (ᴳ- D3)) as (DisjointD1mD3 & DisjointD2mD3) by apply (DisjointNestedLeft D1 D2 (ᴳ- D3) H1).
-    assert (ctx_Disjoint D2 D3) as DisjointD2D3 by apply (DisjointMinusRightBackward D2 D3 DisjointD2mD3).
-    assert (ctx_Disjoint (¹↑ ᴳ· D2) D3) as DisjointsD2D3 by apply (DisjointStimesLeftForward ¹↑ D2 D3 DisjointD2D3).
-    exact (LinOnlyUnionForward (¹↑ ᴳ· D2) D3 LinOnlysD2 LinOnlyD3 DisjointsD2D3).
+  - apply EmptyIsLinOnly.
+  - hauto_ctx.
+  - hauto_ctx.
+  - hauto_ctx.
+  - hauto_ctx.
+  - hauto_ctx.
+  - hauto_ctx.
+  - hauto_ctx.
+  - hauto_ctx.
+  - hauto_ctx.
+  - hauto_ctx.
+  - hauto_ctx.
+  - hauto_ctx.
+  - hauto_ctx.
+  - hauto_ctx.
+  - hauto_ctx.
+  - hauto_ctx.
+  - hauto_ctx.
+  - assert (ctx_LinOnly (¹↑ ᴳ· D2)) by (hauto l: on use: LinOnlyUnionEquiv, LinOnlyStimesEquiv, (mode_IsLinProof (Fin 1))).
+    assert (ctx_Disjoint (D1 ⨄ D2) (ᴳ-D3)) by (apply (hdns_DisjointImpliesDisjoint (D1 ⨄ D2) (ᴳ-D3) C (T1 ⧔ U) U0); tauto).
+    assert (ctx_Disjoint (¹↑ ᴳ· D2) D3) by (sblast use: DisjointNestedLeftEquiv, DisjointMinusRightEquiv, DisjointStimesLeftEquiv).
+    rewrite (LinOnlyUnionEquiv (¹↑ ᴳ· D2) D3). split; tauto.
 Qed.
 
-Lemma tSubLemma : forall (D1 D2 : ctx) (m : mode) (T1 T2 : type) (t' : term) (x : var) (v : val), ctx_DestOnly D2 -> (D2 ⨄ ᴳᵛ{ ᵛ x : m ‗ T1} ⊢ t' : T2) -> (D1 ⊢ ᵥ₎ v : T1) -> (m ᴳ· D1 ⨄ D2 ⊢ t' ᵗ[ x ≔ v] : T2). Proof. Admitted.
+Lemma tSubLemma : forall (D1 D2 : ctx) (m : mode) (T1 T2 : type) (t' : term) (x : var) (v : val), ctx_DestOnly D2 -> (D2 ⨄ ᴳ{ x : m ‗ T1} ⊢ t' : T2) -> (D1 ⊢ ᵥ₎ v : T1) -> (m ᴳ· D1 ⨄ D2 ⊢ t' ᵗ[ x ≔ v] : T2). Proof. Admitted.
 
 Theorem Preservation : forall (C C' : ectxs) (t t' : term) (T : type), ⊢ C ʲ[t] : T /\
   C ʲ[t] ⟶ C' ʲ[t'] -> ⊢ C' ʲ[t'] : T.
@@ -99,101 +110,90 @@ Proof.
     - (* Sem-eterm-AppFoc1 *)
       inversion Tyt; subst.
       rename Tyt into TyApp, Tyt0 into Tyt, P1 into D1, P2 into D2, T into T2.
-      assert (ctx_DestOnly (m ᴳ· D1) /\ ctx_DestOnly D2)
-        as (DestOnlymD1 & DestOnlyD2)
-        by apply (DestOnlyUnionBackward (m ᴳ· D1) D2 DestOnlyD).
-      assert (ctx_DestOnly D1)
-        as DestOnlyD1
-        by apply (DestOnlyStimesBackward m D1 DestOnlymD1).
-      assert (ctx_LinOnly (m ᴳ· D1 ⨄ D2))
-        as LinOnlyD
-        by apply (Ty_ectxs_DLin (m ᴳ· D1 ⨄ D2) C T2 U0 TyC).
-      assert (ctx_LinOnly (m ᴳ· D1) /\ ctx_LinOnly D2 /\ ctx_Disjoint (m ᴳ· D1) D2) 
-        as (LinOnlymD1 & LinOnlyD2 & DisjointmD1D2)
-        by apply (LinOnlyUnionBackward (m ᴳ· D1) D2 LinOnlyD).
-      assert (ctx_Disjoint D1 D2)
-        as DisjointD1D2
-        by apply (DisjointStimesLeftBackward m D1 D2 DisjointmD1D2).
-      assert (ctx_LinOnly D1 /\ mode_IsLin m)
-        as (LinOnlyD1 & IsLinm)
-        by apply (LinOnlyStimesBackward m D1 LinOnlymD1).
-      assert (D1 ⊣ C ∘ ⬜≻ u : T1 ↣ U0)
-        as TyCc
-        by apply (Ty_ectxs_AppFoc1 D1 C u T1 U0 D2 m T2 DisjointD1D2 DestOnlyD1 DestOnlyD2 (IsLinIsValid m IsLinm) (LinOnlyIsValid D2 LinOnlyD2) TyC Tyu).
-      exact (Ty_eterm_ClosedEterm (C ∘ ⬜≻ u) t U0 D1 T1 (LinOnlyIsValid D1 LinOnlyD1) DestOnlyD1 TyCc Tyt).
+      assert (ctx_LinOnly (m ᴳ· D1 ⨄ D2)) as LinOnlyD by (apply (Ty_ectxs_LinOnlyD (m ᴳ· D1 ⨄ D2) C T2 U0); tauto).
+      constructor 1 with (D := D1) (T := T1) (t := t); swap 1 3. constructor 2 with (D2 := D2) (m := m) (u := u) (T2 := T2).
+      all: hauto_ctx.
     - (* Sem-eterm-AppUnfoc1 *)
-      inversion Tyt; subst. rename H2 into TyRv, TyC into TyCc, D into D1, ValidD into ValidD1, DestOnlyD into DestOnlyD1. clear H0.
+      inversion Tyt; subst. rename H2 into TyRv, TyC into TyCc, D into D1, ValidOnlyD into ValidOnlyD1, DestOnlyD into DestOnlyD1. clear H0.
       inversion TyCc; subst. clear DestOnlyD0. rename T into T1.
-      assert (m ᴳ· D1 ⨄ D2 ⊢ ᵥ₎ v ≻ u : T2)
-        as TyApp
-        by apply (Ty_term_App m D1 D2 (ᵥ₎ v) u T2 T1 Tyt Tyu).
-      assert (ctx_LinOnly (m ᴳ· D1 ⨄ D2))
-        as LinOnlymD1D2
-        by apply (Ty_ectxs_DLin (m ᴳ· D1 ⨄ D2) C T2 U0 TyC).
-      assert (ctx_IsValid (m ᴳ· D1 ⨄ D2))
-        as ValidmD1D2
-        by apply (LinOnlyIsValid (m ᴳ· D1 ⨄ D2) LinOnlymD1D2).
-      assert (ctx_DestOnly (m ᴳ· D1))
-        as DestOnlymD
-        by apply (DestOnlyStimesForward m D1 DestOnlyD1).
-      assert (ctx_DestOnly (m ᴳ· D1 ⨄ D2))
-        as DestOnlymD1D2
-        by apply (DestOnlyUnionForward (m ᴳ· D1) D2 DestOnlymD DestOnlyD2).
-      exact (Ty_eterm_ClosedEterm C (ᵥ₎ v ≻ u) U0 (m ᴳ· D1 ⨄ D2) T2 ValidmD1D2 DestOnlymD1D2 TyC TyApp).
+      assert (ctx_LinOnly (m ᴳ· D1 ⨄ D2)) as LinOnlyD by (apply (Ty_ectxs_LinOnlyD (m ᴳ· D1 ⨄ D2) C T2 U0); tauto).
+      assert (m ᴳ· D1 ⨄ D2 ⊢ ᵥ₎ v ≻ u : T2) as TyApp by (apply (Ty_term_App m D1 D2 (ᵥ₎ v) u T2 T1); tauto).
+      constructor 1 with (D := (m ᴳ· D1 ⨄ D2)) (T := T2) (t := ᵥ₎ v ≻ u). all: hauto_ctx.
     - (* Sem-eterm-AppFoc2 *)
       inversion Tyt; subst.
       rename Tyt into TyApp, Tyt0 into Tyt, P1 into D1, P2 into D2, T into T2.
-      assert (ctx_DestOnly (m ᴳ· D1) /\ ctx_DestOnly D2)
-        as (DestOnlymD1 & DestOnlyD2)
-        by apply (DestOnlyUnionBackward (m ᴳ· D1) D2 DestOnlyD).
-      assert (ctx_DestOnly D1)
-        as DestOnlyD1
-        by apply (DestOnlyStimesBackward m D1 DestOnlymD1).
-      assert (ctx_LinOnly (m ᴳ· D1 ⨄ D2))
-        as LinOnlyD
-        by apply (Ty_ectxs_DLin (m ᴳ· D1 ⨄ D2) C T2 U0 TyC).
-      assert (ctx_LinOnly (m ᴳ· D1) /\ ctx_LinOnly D2 /\ ctx_Disjoint (m ᴳ· D1) D2) 
-        as (LinOnlymD1 & LinOnlyD2 & DisjointmD1D2)
-        by apply (LinOnlyUnionBackward (m ᴳ· D1) D2 LinOnlyD).
-      assert (ctx_Disjoint D1 D2)
-        as DisjointD1D2
-        by apply (DisjointStimesLeftBackward m D1 D2 DisjointmD1D2).
-      assert (ctx_LinOnly D1 /\ mode_IsLin m)
-        as (LinOnlyD1 & IsLinm)
-        by apply (LinOnlyStimesBackward m D1 LinOnlymD1).
-      assert (D2 ⊣ C ∘ v ≻⬜ : (T1 ⁔ m → T2) ↣ U0)
-        as TyCc
-        by apply (Ty_ectxs_AppFoc2 D2 C v T1 m T2 U0 D1 DisjointD1D2 DestOnlyD1 DestOnlyD2 (LinOnlyIsValid (m ᴳ· D1) LinOnlymD1) TyC Tyt).
-      exact (Ty_eterm_ClosedEterm (C ∘ v ≻⬜) u U0 D2 (T1 ⁔ m → T2) (LinOnlyIsValid D2 LinOnlyD2) DestOnlyD2 TyCc Tyu).
+      assert (ctx_LinOnly (m ᴳ· D1 ⨄ D2)) as LinOnlyD by (apply (Ty_ectxs_LinOnlyD (m ᴳ· D1 ⨄ D2) C T2 U0); tauto).
+      constructor 1 with (D := D2) (T := T1 ⁔ m → T2) (t := u); swap 1 3. constructor 3 with (D1 := D1) (m := m) (v := v) (T1 := T1) (T2 := T2). all: hauto_ctx.
     - (* Sem-eterm-AppUnfoc2 *)
-      inversion Tyt; subst. rename H2 into TyRv, TyC into TyCc, D into D2, ValidD into ValidD2, DestOnlyD into DestOnlyD2. clear H0.
+      inversion Tyt; subst. rename H2 into TyRv, TyC into TyCc, D into D2, ValidOnlyD into ValidOnlyD2, DestOnlyD into DestOnlyD2. clear H0.
       inversion TyCc; subst. clear DestOnlyD0. rename Tyt into Tyu, Tyv into Tyt.
-      assert (m ᴳ· D1 ⨄ D2 ⊢ ᵥ₎ v ≻ ᵥ₎ v' : T2)
-        as TyApp
-        by apply (Ty_term_App m D1 D2 (ᵥ₎ v) (ᵥ₎ v') T2 T1 Tyt Tyu).
-      assert (ctx_LinOnly (m ᴳ· D1 ⨄ D2))
-        as LinOnlymD1D2
-        by apply (Ty_ectxs_DLin (m ᴳ· D1 ⨄ D2) C T2 U0 TyC).
-      assert (ctx_IsValid (m ᴳ· D1 ⨄ D2))
-        as ValidmD1D2
-        by apply (LinOnlyIsValid (m ᴳ· D1 ⨄ D2) LinOnlymD1D2).
-      assert (ctx_DestOnly (m ᴳ· D1))
-        as DestOnlymD
-        by apply (DestOnlyStimesForward m D1 DestOnlyD1).
-      assert (ctx_DestOnly (m ᴳ· D1 ⨄ D2))
-        as DestOnlymD1D2
-        by apply (DestOnlyUnionForward (m ᴳ· D1) D2 DestOnlymD DestOnlyD2).
-      exact (Ty_eterm_ClosedEterm C ((ᵥ₎ v) ≻ (ᵥ₎ v')) U0 (m ᴳ· D1 ⨄ D2) T2 ValidmD1D2 DestOnlymD1D2 TyC TyApp).
+      assert (m ᴳ· D1 ⨄ D2 ⊢ ᵥ₎ v ≻ ᵥ₎ v' : T2) as TyApp by (apply (Ty_term_App m D1 D2 (ᵥ₎ v) (ᵥ₎ v') T2 T1); tauto).
+      assert (ctx_LinOnly (m ᴳ· D1 ⨄ D2)) as LinOnlyD by (apply (Ty_ectxs_LinOnlyD (m ᴳ· D1 ⨄ D2) C T2 U0); tauto).
+      constructor 1 with (D := (m ᴳ· D1 ⨄ D2)) (T := T2) (t := (ᵥ₎ v) ≻ (ᵥ₎ v')). all: hauto_ctx.
     - (* Sem-eterm-AppRed *)
       inversion Tyt; subst.
-      assert (m = m0) as Eqmm0.
-        inversion_clear Tyu. inversion_clear H0. tauto.
-      rewrite <- Eqmm0 in Tyu, Tyt, TyC, DestOnlyD, ValidD. clear Eqmm0. clear m0. rename P1 into D1, P2 into D2. rename Tyt into TyApp, Tyt0 into Tyt, T into T2, t into t'.
+      assert (m = m0) as Eqmm0 by (inversion_clear Tyu; inversion_clear H0; tauto).
+      rewrite <- Eqmm0 in Tyu, Tyt, TyC, DestOnlyD, ValidOnlyD. clear Eqmm0. clear m0. rename P1 into D1, P2 into D2. rename Tyt into TyApp, Tyt0 into Tyt, T into T2, t into t'.
       inversion Tyu; subst. clear H0. rename H2 into TyRv'.
       inversion TyRv'; subst. rename Tyt0 into Tyt'. rename H1 into DestOnlyD2.
-      assert (m ᴳ· D1 ⨄ D2 ⊢ t' ᵗ[ x ≔ v] : T2)
-        as Tytpsub
-        by (apply (tSubLemma D1 D2 m T1 T2 t' x v DestOnlyD2 Tyt' Tyt)).
-      exact (Ty_eterm_ClosedEterm C (t' ᵗ[ x ≔ v]) U0 (m ᴳ· D1 ⨄ D2) T2 ValidD DestOnlyD TyC Tytpsub).
+      assert (m ᴳ· D1 ⨄ D2 ⊢ t' ᵗ[ x ≔ v] : T2) as Tytpsub by (apply (tSubLemma D1 D2 m T1 T2 t' x v); tauto).
+      constructor 1 with (D := (m ᴳ· D1 ⨄ D2)) (T := T2) (t := t' ᵗ[ x ≔ v]). all: hauto_ctx.
+    - (* Sem-eterm-PatUFoc *)
+      inversion Tyt; subst.
+      rename Tyt into TyPat, Tyt0 into Tyt, P1 into D1, P2 into D2, T into T2.
+      assert (ctx_LinOnly (D1 ⨄ D2)) as LinOnlyD by (apply (Ty_ectxs_LinOnlyD (D1 ⨄ D2) C T2 U0); tauto).
+      constructor 1 with (D := D1) (T := 𝟏) (t := t); swap 1 3. constructor 4 with (D2 := D2) (U := T2) (u := u). all: hauto_ctx.
+    - (* Sem-eterm-PatUUnfoc *)
+      inversion Tyt; subst. rename H2 into TyRv, TyC into TyCc, D into D1, ValidOnlyD into ValidOnlyD1, DestOnlyD into DestOnlyD1. clear H0.
+      inversion TyCc; subst. clear DestOnlyD0. rename U into T2.
+      assert (ctx_LinOnly (D1 ⨄ D2)) as LinOnlyD by (apply (Ty_ectxs_LinOnlyD (D1 ⨄ D2) C T2 U0); tauto).
+      assert (D1 ⨄ D2 ⊢ ᵥ₎ v ᵗ; u : T2) as TyPat by (apply (Ty_term_PatU D1 D2 (ᵥ₎ v) u T2); tauto).
+      constructor 1 with (D := (D1 ⨄ D2)) (T := T2) (t := ᵥ₎ v ᵗ; u). all: hauto_ctx.
+    - (* Sem-eterm-PatURed *)
+      inversion Tyt; subst.
+      rename P1 into D1, P2 into D2. rename Tyt into TyPat, Tyt0 into Tyt, T into T2.
+      inversion Tyt; subst. rename H0 into DestOnlyD1, H2 into TyRv.
+      inversion TyRv; subst.
+      constructor 1 with (D := D2) (T := T2) (t := u). all: hauto_ctx.
+    - (* Sem-eterm-PatSFoc *)
+      inversion Tyt; subst.
+      rename Tyt into TyPat, Tyt0 into Tyt, P1 into D1, P2 into D2, T into U.
+      assert (ctx_LinOnly (m ᴳ· D1 ⨄ D2)) as LinOnlyD by (apply (Ty_ectxs_LinOnlyD (m ᴳ· D1 ⨄ D2) C U U0); tauto).
+      constructor 1 with (D := D1) (T := (T1 ⨁ T2)) (t := t) ; swap 1 3. constructor 5 with (D1 := D1) (D2 := D2) (m := m) (u1 := u1) (x1 := x1) (u2 := u2) (x2 := x2) (U := U). all: hauto_ctx.
+    - (* Sem-eterm-PatSUnfoc *)
+      inversion Tyt; subst. rename H2 into TyRv, TyC into TyCc, D into D1, ValidOnlyD into ValidOnlyD1, DestOnlyD into DestOnlyD1. clear H0.
+      inversion TyCc; subst. clear DestOnlyD0.
+      assert (ctx_LinOnly (m ᴳ· D1 ⨄ D2)) as LinOnlyD by (apply (Ty_ectxs_LinOnlyD (m ᴳ· D1 ⨄ D2) C U U0); tauto).
+      assert (m ᴳ· D1 ⨄ D2 ⊢ ᵥ₎ v ≻caseˢ m {Inl x1 ⟼ u1, Inr x2 ⟼ u2} : U) as TyPat by (apply (Ty_term_PatS m D1 D2 (ᵥ₎ v) x1 u1 x2 u2 U T1 T2); hauto_ctx).
+      constructor 1 with (D := (m ᴳ· D1 ⨄ D2)) (T := U) (t := ᵥ₎ v ≻caseˢ m {Inl x1 ⟼ u1, Inr x2 ⟼ u2}). all: hauto_ctx.
+    - (* Sem-eterm-PatLRed *)
+      inversion Tyt; subst.
+      rename P1 into D1, P2 into D2. rename Tyt into TyPat, Tyt0 into Tyt, T into U.
+      inversion Tyt; subst. rename H0 into DestOnlyD1, H2 into TyRInlv.
+      inversion TyRInlv; subst.
+      assert (D1 ⊢ ᵥ₎ v : T1) as Tyt' by (apply Ty_term_Val; tauto).
+      assert (m ᴳ· D1 ⨄ D2 ⊢ u1 ᵗ[ x1 ≔ v] : U) as Tyusub by (apply (tSubLemma D1 D2 m T1 U u1 x1 v); hauto_ctx).
+      constructor 1 with (D := (m ᴳ· D1 ⨄ D2)) (T := U) (t := u1 ᵗ[ x1 ≔ v]). all: hauto_ctx.
+    - (* Sem-eterm-PatRRed *)
+      inversion Tyt; subst.
+      rename P1 into D1, P2 into D2. rename Tyt into TyPat, Tyt0 into Tyt, T into U.
+      inversion Tyt; subst. rename H0 into DestOnlyD1, H2 into TyRInlv.
+      inversion TyRInlv; subst.
+      assert (D1 ⊢ ᵥ₎ v : T2) as Tyt' by (apply Ty_term_Val; tauto).
+      assert (m ᴳ· D1 ⨄ D2 ⊢ u2 ᵗ[ x2 ≔ v] : U) as Tyusub by (apply (tSubLemma D1 D2 m T2 U u2 x2 v); hauto_ctx).
+      constructor 1 with (D := (m ᴳ· D1 ⨄ D2)) (T := U) (t := u2 ᵗ[ x2 ≔ v]). all: hauto_ctx.
+    - (* Sem-eterm-PatPFoc *)
+      inversion Tyt; subst.
+      rename Tyt into TyPat, Tyt0 into Tyt, P1 into D1, P2 into D2, T into U.
+      assert (ctx_LinOnly (m ᴳ· D1 ⨄ D2)) as LinOnlyD by (apply (Ty_ectxs_LinOnlyD (m ᴳ· D1 ⨄ D2) C U U0); tauto).
+      constructor 1 with (D := D1) (T := (T1 ⨂ T2)) (t := t) ; swap 1 3. constructor 6 with (D1 := D1) (D2 := D2) (u := u) (x1 := x1) (x2 := x2) (U := U). all: hauto_ctx.
+    - (* Sem-eterm-PatPUnfoc *)
+      inversion Tyt; subst. rename H2 into TyRv, TyC into TyCc, D into D1, ValidOnlyD into ValidOnlyD1, DestOnlyD into DestOnlyD1. clear H0.
+      inversion TyCc; subst. clear DestOnlyD0.
+      assert (ctx_LinOnly (m ᴳ· D1 ⨄ D2)) as LinOnlyD by (apply (Ty_ectxs_LinOnlyD (m ᴳ· D1 ⨄ D2) C U U0); tauto).
+      assert (m ᴳ· D1 ⨄ D2 ⊢ ᵥ₎ v ≻caseᵖ m ᵗ(x1 , x2) ⟼ u : U) as TyPat by (apply (Ty_term_PatP m D1 D2 (ᵥ₎ v) x1 x2 u U T1 T2); hauto_ctx).
+      constructor 1 with (D := (m ᴳ· D1 ⨄ D2)) (T := U) (t := ᵥ₎ v ≻caseᵖ m ᵗ(x1 , x2) ⟼ u). all: hauto_ctx.
     - give_up.
 Admitted.
+
+
